\documentclass{article}
\usepackage{amsmath}
\begin{document}
\(Constant.OUT1^{[s+1]} = 5;\)\\
\(Constant2.OUT1^{[s+1]} = 2;\)\\
\(Negator.IN1^{[s+1]} = Constant.OUT1^{[s+1]};\)\\
\(Negator.OUT1^{[s+1]} = -Negator.IN1^{[s+1]};\)\\
\(Inverter.IN1^{[s+1]} = Negator.OUT1^{[s+1]};\)\\
\(Inverter.OUT1^{[s+1]} = \dfrac{1}{Inverter.IN1^{[s+1]}};\)\\
\(Adder.IN1^{[s+1]} = Inverter.OUT1^{[s+1]};\)\\
\(Adder.IN2^{[s+1]} = Constant.OUT1^{[s+1]};\)\\
\(Adder.OUT1^{[s+1]} = Adder.IN1^{[s+1]} + Adder.IN2^{[s+1]};\)\\
\(Product.IN1^{[s+1]} = Adder.OUT1^{[s+1]};\)\\
\(Product.IN2^{[s+1]} = Constant.OUT1^{[s+1]};\)\\
\(Product.OUT1^{[s+1]} = Product.IN1^{[s+1]} * Product.IN2^{[s+1]};\)\\
\(Generic.IN1^{[s+1]} = Product.OUT1^{[s+1]};\)\\
\(Generic.OUT1^{[s+1]} = sin(Generic.IN1)^{[s+1]}\)\\
\(Root.IN1^{[s+1]} = Generic.OUT1^{[s+1]};\)\\
\(Root.IN2^{[s+1]} = Constant2.OUT1^{[s+1]};\)\\
\(Root.OUT1^{[s+1]} = \sqrt[Root.IN2]{Root.IN1}^{[s+1]};\)\\
\(Modulo.IN1^{[s+1]} = Root.OUT1^{[s+1]};\)\\
\(Modulo.IN2^{[s+1]} = Constant.OUT1^{[s+1]};\)\\
\(Modulo.OUT1^{[s+1]} = Modulo.IN1^{[s+1]} \% Modulo.OUT1^{[s+1]};\)\\
\(Delay.OUT1^{[s+1]} = Delay.IN1^{[s]};\)\\
\(Delay.OUT1^{[0]} = Delay.IN2^{[s+1]};\)\\
\end{document}